Prove that deleting on bootstraped heaps preserves ordering
This commit contains a lot of auxilliary lemmas regarding the conservation of ordering on bootstraped heaps when we apply functions of our first implementation on the underlying skew binomial heap.
It also defines and proves the relation between the result of delete_min and find_min on bootstraped heaps, which was needed to prove that delete_min preserves the ordering of a boostraped heap.

translator/okasaki-examples/SkewBinomialHeapScript.sml
@@ -39,7 +39,7 @@ val skew_link_def = Define `
         (if geq x' x
          then (Sbnode x r (x'::a) c)
          else (Sbnode x' r (x::a) c))
-  `;
+`;
 
 val tree_to_bag_def = Define `
   (tree_to_bag (Sbnode x r a []) = (BAG_INSERT x (list_to_bag a))) /\
@@ -192,7 +192,7 @@ val b_delete_min_def = Define `
   (b_delete_min _ Bsbempty = NONE) /\
   (b_delete_min geq (Bsbheap _ c) =
     if c = [] then (SOME Bsbempty) else
-co    let min = THE (find_min (b_heap_comparison geq) c) in
+    let min = THE (find_min (b_heap_comparison geq) c) in
     let rest = THE (delete_min (b_heap_comparison geq) c) in
     let smallest_root = b_root min in
     let smallest_children = b_children min in
@@ -229,7 +229,10 @@ val is_b_heap_ordered_def = Define `
      is_b_heap_ordered3 geq a /\
      is_b_heap_ordered4 geq c)) /\
   (is_b_heap_ordered3 geq [] = T) /\
-  (is_b_heap_ordered3 geq (e::es) = (is_b_heap_ordered geq e /\ is_b_heap_ordered3 geq es)) /\
+  (is_b_heap_ordered3 geq (e::es) = (
+     e <> Bsbempty /\
+     is_b_heap_ordered geq e /\
+     is_b_heap_ordered3 geq es)) /\
   (is_b_heap_ordered4 geq [] = T) /\
   (is_b_heap_ordered4 geq (t::ts) = (is_tree_ordered (b_heap_comparison geq) t /\
                                      is_b_heap_ordered2 geq t /\
@@ -243,7 +246,7 @@ val TotalPreOrder = Define `
 
 (* Useful lemmas *)
 Theorem rank_irrelevance_bag:
-  !root r1 r2 aux ch. tree_to_bag (Sbnode root r1 aux ch) = tree_to_bag (Sbnode root r2 aux ch)
+ !root r1 r2 aux ch. tree_to_bag (Sbnode root r1 aux ch) = tree_to_bag (Sbnode root r2 aux ch)
 Proof
   Induct_on `ch` \\ rw[tree_to_bag_def]
 QED;
@@ -388,6 +391,13 @@ Proof
   Induct_on `h`
   >- rw[b_heap_to_bag_def]
   >- rw[b_heap_to_bag_def]
+QED;
+
+Theorem equiv_order4_order1:
+  !geq h. is_b_heap_ordered4 geq h = is_b_heap_ordered1 geq h
+Proof
+  Induct_on `h` \\
+  rw[is_b_heap_ordered_def]
 QED;
 
 Theorem tree_link_choice:
@@ -1396,10 +1406,11 @@ Proof
                      metis_tac[transitive_def]))))
      >- (imp_res_tac link_b_order \\ fs[is_b_heap_ordered_def])
      >- (imp_res_tac link_b_order \\ fs[is_b_heap_ordered_def])
+     >- (imp_res_tac link_b_order \\ fs[is_b_heap_ordered_def])
      >- (imp_res_tac link_b_order \\ fs[is_b_heap_ordered_def]))
   >- (rw[root_def, rank_def, aux_def, children_def, is_b_heap_ordered_def]
-      >- (imp_res_tac link_b_order \\ fs[is_b_heap_ordered_def] )
-      >- (imp_res_tac link_b_order \\ fs[is_b_heap_ordered_def] )
+      >- (imp_res_tac link_b_order \\ fs[is_b_heap_ordered_def])
+      >- (imp_res_tac link_b_order \\ fs[is_b_heap_ordered_def])
       >- (imp_res_tac link_b_order \\
           fs[is_b_heap_ordered_def] \\
           rw[b_heap_to_bag_def] \\
@@ -1441,6 +1452,44 @@ Proof
               rw[])
           >- rw[leaf_def, is_b_heap_ordered_def, is_tree_ordered_def,
 	        list_to_bag_def, b_heap_to_bag_def]))
+QED;
+
+Theorem insert_list_b_order:
+  !geq l h. TotalPreOrder geq /\
+            is_b_heap_ordered1 geq h /\
+            is_b_heap_ordered3 geq l ==>
+            is_b_heap_ordered1 geq (insert_list (b_heap_comparison geq) l h)
+Proof
+  Induct_on `l`
+  >- rw[insert_list_def]
+  >- (rw[insert_list_def] \\
+      fs[is_b_heap_ordered_def] \\
+      res_tac \\
+      imp_res_tac insert_b_order)
+QED;
+
+Theorem app_b_order:
+  !geq l1 l2. TotalPreOrder geq /\
+              is_b_heap_ordered1 geq l1 /\
+              is_b_heap_ordered1 geq l2 ==>
+              is_b_heap_ordered1 geq (l1 ++ l2)
+Proof
+  Induct_on `l1`
+  >- rw[]
+  >- rw[is_b_heap_ordered_def]
+QED;
+
+Theorem reverse_b_order:
+  !geq l. TotalPreOrder geq /\
+          is_b_heap_ordered1 geq l ==>
+          is_b_heap_ordered1 geq (REVERSE l)
+Proof
+  Induct_on `l`
+  >- rw[]
+  >- (rw[] \\
+      fs[is_b_heap_ordered_def] \\
+      `is_b_heap_ordered1 geq [h]` by rw[is_b_heap_ordered_def] \\
+      rw[app_b_order])
 QED;
 
 Theorem b_merge_order:
@@ -1593,8 +1642,254 @@ Proof
   >- (rw[merge_def, b_merge_tree_bag1, b_normalize_bag1])
 QED;
 
+Theorem get_min_b_order:
+  !geq h smallest rest. TotalPreOrder geq /\
+                        h <> [] /\
+                        is_b_heap_ordered1 geq h /\
+                        (smallest, rest) = get_min (b_heap_comparison geq) h ==>
+                        is_b_heap_ordered2 geq smallest /\
+                        is_b_heap_ordered1 geq rest
+Proof
+  Induct_on `h`
+  >- rw[]
+  >- (Cases_on `h`
+      >- rw[is_b_heap_ordered_def, get_min_def]
+      >- (rw[is_b_heap_ordered_def, get_min_def] \\
+          Cases_on `get_min (b_heap_comparison geq) (h'::t)` \\
+          fs[] \\
+          `(q,r) = get_min (b_heap_comparison geq) (h'::t)` by rw[]
+	  >- (Cases_on `(b_heap_comparison geq) (root q) (root h)`
+              >- fs[]
+	      >- (fs[] \\
+                  res_tac))
+          >- (Cases_on `(b_heap_comparison geq) (root q) (root h)`
+              >- fs[is_b_heap_ordered_def]
+	      >- (res_tac \\
+                  fs[is_b_heap_ordered_def]))))
+QED;
+
+Theorem binomial_insert_b_order:
+  !geq t h. TotalPreOrder geq /\
+            is_b_heap_ordered1 geq h /\
+            is_b_heap_ordered2 geq t ==>
+            is_b_heap_ordered1 geq (binomial_insert (b_heap_comparison geq) t h)
+Proof
+  Induct_on `h`
+  >- rw[is_b_heap_ordered_def, is_tree_ordered_def, binomial_insert_def,
+     tree_b_ordered_is_ordered]
+  >- (Induct_on `h`
+      >- (rw[is_b_heap_ordered_def, is_tree_ordered_def, binomial_insert_def] \\
+          Cases_on `rank t < rank h`
+          >- rw[is_b_heap_ordered_def]
+	  >- (rw[] \\
+              Cases_on `tree_link (b_heap_comparison geq) t h` \\
+              imp_res_tac link_b_order \\
+              rw[is_b_heap_ordered_def]))
+      >- (rw[is_b_heap_ordered_def] \\
+          rw[binomial_insert_def, is_b_heap_ordered_def]
+          >- fs[tree_b_ordered_is_ordered]
+          >- (imp_res_tac tree_b_ordered_is_ordered \\
+              imp_res_tac b_comparison_total_pre_order \\
+              rw[tree_link_order])
+          >- (Cases_on `tree_link (b_heap_comparison geq) t h''` \\
+              imp_res_tac link_b_order)
+          >- (Cases_on `tree_link (b_heap_comparison geq) t h''` \\
+              imp_res_tac link_b_order \\
+              imp_res_tac tree_b_ordered_is_ordered \\
+              res_tac \\
+	      fs[binomial_insert_def] \\
+              fs[rank_def] \\
+              rfs[])))
+QED;
+
+Theorem normalize_b_order:
+  !geq h. TotalPreOrder geq /\
+          is_b_heap_ordered1 geq h ==>
+          is_b_heap_ordered1 geq (normalize (b_heap_comparison geq) h)
+Proof
+  Cases_on `h` \\
+  rw[is_b_heap_ordered_def, normalize_def, binomial_insert_b_order]
+QED;
+
+Theorem merge_tree_b_order:
+  !geq h1 h2. TotalPreOrder geq /\
+              is_b_heap_ordered1 geq h1 /\
+              is_b_heap_ordered1 geq h2 ==>
+              is_b_heap_ordered1 geq (merge_tree (b_heap_comparison geq) h1 h2)
+Proof
+  Induct_on `h2`
+  >- rw[merge_tree_def, is_b_heap_ordered_def]
+  >- (Induct_on `h1`
+      >- rw[merge_tree_left_cancel, is_b_heap_ordered_def]
+      >- (rw[merge_tree_def]
+	  >- (rw[is_b_heap_ordered_def]
+	      >- fs[is_b_heap_ordered_def]
+	      >- fs[is_b_heap_ordered_def]
+	      >- fs[is_b_heap_ordered_def])
+          >- (rw[is_b_heap_ordered_def]
+              >- fs[is_b_heap_ordered_def, tree_b_ordered_is_ordered]
+	      >- fs[is_b_heap_ordered_def]
+	      >- fs[is_b_heap_ordered_def])
+          >- (fs[is_b_heap_ordered_def] \\
+              `is_b_heap_ordered1 geq (merge_tree (b_heap_comparison geq) h1 h2)`
+              by res_tac \\
+              Cases_on `tree_link (b_heap_comparison geq) h h'` \\
+              imp_res_tac link_b_order \\
+              rw[binomial_insert_b_order])))
+QED;
+
+Theorem merge_b_order:
+  !geq h1 h2. TotalPreOrder geq /\
+              is_b_heap_ordered1 geq h1 /\
+              is_b_heap_ordered1 geq h2 ==>
+              is_b_heap_ordered1 geq (merge (b_heap_comparison geq) h1 h2)
+Proof
+  Cases_on `h2`
+  >- rw[is_b_heap_ordered_def, merge_def, normalize_def,
+        merge_tree_def, normalize_b_order]
+  >- rw[is_b_heap_ordered_def, merge_def, normalize_def,
+	 merge_tree_def, normalize_b_order, binomial_insert_b_order,
+	 normalize_b_order, merge_tree_b_order]
+QED;
+
+Theorem delete_b_order:
+  !geq h. TotalPreOrder geq /\
+           h <> [] /\
+           is_b_heap_ordered1 geq h ==>
+           is_b_heap_ordered1 geq (THE (delete_min (b_heap_comparison geq) h))
+Proof
+  Induct_on `h`
+  >- rw[]
+  >- (rw[delete_min_def] \\
+      Cases_on `get_min (b_heap_comparison geq) (h'::h)` \\
+      `(q,r) = get_min (b_heap_comparison geq) (h'::h)` by rw[] \\
+      `(h'::h) <> []` by rw[] \\
+      imp_res_tac get_min_b_order \\
+      simp[] \\
+      Cases_on `q` \\
+      fs[is_b_heap_ordered_def] \\
+      rw[aux_def, children_def] \\
+      fs[equiv_order4_order1] \\
+      rw[normalize_b_order, reverse_b_order, merge_tree_b_order,
+	 insert_list_b_order])
+QED;
+
+Theorem find_min_b_order:
+  !geq h. is_b_heap_ordered1 geq h /\
+          h <> [] ==>
+          is_b_heap_ordered geq (THE (find_min (b_heap_comparison geq) h))
+Proof
+  Induct_on `h`
+  >- rw[]
+  >- (Cases_on `h`
+      >- (rw[is_b_heap_ordered_def, find_min_def] \\
+          Cases_on `h` \\
+          fs[root_def, is_b_heap_ordered_def])
+      >- (rw[find_min_def, is_b_heap_ordered_def] \\
+          Cases_on `find_min (b_heap_comparison geq) (h'::t)`
+          >- (`(h'::t) <> []` by rw[] \\
+              imp_res_tac find_min_exists)
+          >- (rw[]
+	      >- (Cases_on `h` \\
+                  fs[root_def, is_b_heap_ordered_def])
+              >- (res_tac \\
+                  metis_tac[THE_DEF]))))
+QED;
+
+Theorem find_min_b_non_empty:
+  !geq h. is_b_heap_ordered1 geq h /\
+          h <> [] ==>
+          THE (find_min (b_heap_comparison geq) h) <> Bsbempty
+Proof
+  Induct_on `h`
+  >- rw[]
+  >- (Cases_on `h`
+      >- (rw[find_min_def, is_b_heap_ordered_def] \\
+          Cases_on `h` \\
+          fs[root_def, is_b_heap_ordered_def])
+      >- (rw[find_min_def, is_b_heap_ordered_def] \\
+          Cases_on `find_min (b_heap_comparison geq) (h'::t)`
+          >- (`h'::t <> []` by rw[] \\
+              imp_res_tac find_min_exists)
+          >- (rw[]
+              >- (Cases_on `h` \\
+                  fs[root_def, is_b_heap_ordered_def])
+              >- (res_tac \\
+                  metis_tac[THE_DEF]))))
+QED;
+
+Theorem b_find_delete_min:
+  !geq h. TotalPreOrder geq /\
+          is_b_heap_ordered1 geq h /\
+          h <> [] ==>
+          BAG_EVERY (\y. geq y (b_root (THE (find_min (b_heap_comparison geq) h))))
+                    (b_heap_to_bag1 geq (THE (delete_min (b_heap_comparison geq) h)))
+Proof
+  rw[] \\
+  imp_res_tac heap_b_ordered_is_ordered \\
+  imp_res_tac b_comparison_total_pre_order \\
+  imp_res_tac find_min_correct' \\
+  rpt (WEAKEN_TAC is_forall) \\
+  imp_res_tac delete_min_order \\
+  rpt (WEAKEN_TAC is_forall) \\
+  imp_res_tac delete_min_correct \\
+  rpt (WEAKEN_TAC is_forall) \\
+  fs[] \\
+  imp_res_tac find_min_b_order \\
+  imp_res_tac find_min_b_non_empty \\
+  imp_res_tac b_heap_bag1 \\
+  imp_res_tac delete_b_order \\
+  res_tac
+QED;
+
+Theorem b_delete_min_order:
+  !geq h. TotalPreOrder geq /\
+          h <> Bsbempty /\
+          is_b_heap_ordered geq h ==>
+          is_b_heap_ordered geq (THE (b_delete_min geq h))
+Proof
+  rpt strip_tac \\
+  Cases_on `h`
+  >- rw[]
+  >- (fs[is_b_heap_ordered_def] \\
+      rw[b_delete_min_def]
+      >- rw[is_b_heap_ordered_def]
+      >- (rw[is_b_heap_ordered_def]
+	  >- (rw[b_merge_bag1, b_find_delete_min] \\
+              Cases_on `find_min (b_heap_comparison geq) l`
+              >- imp_res_tac find_min_exists
+	      >- (Cases_on `x`
+                  >- (imp_res_tac find_min_b_non_empty \\
+                      rfs[THE_DEF])
+                  >- (rw[THE_DEF, b_root_def, b_children_def] \\
+                      imp_res_tac find_min_b_order \\
+                      rfs[is_b_heap_ordered_def])))
+          >- (Cases_on `find_min (b_heap_comparison geq) l`
+              >- imp_res_tac find_min_exists
+	      >- (Cases_on `x`
+                  >- (imp_res_tac find_min_b_non_empty \\
+                      rfs[THE_DEF])
+                  >- (rw[THE_DEF, b_root_def, b_children_def] \\
+                      imp_res_tac find_min_b_order \\
+                      rfs[is_b_heap_ordered_def] \\
+                      imp_res_tac heap_b_ordered_is_ordered \\
+		      imp_res_tac b_comparison_total_pre_order \\
+                      rw[merge_order, delete_min_order])))
+          >- (imp_res_tac delete_b_order \\
+              Cases_on `find_min (b_heap_comparison geq) l`
+              >- imp_res_tac find_min_exists
+	      >- (Cases_on `x`
+                  >- (imp_res_tac find_min_b_non_empty \\
+                      rfs[THE_DEF])
+                  >- (rw[THE_DEF, b_children_def] \\
+                      imp_res_tac find_min_b_order \\
+                      rfs[is_b_heap_ordered_def] \\
+                      imp_res_tac b_comparison_total_pre_order \\
+                      rw[merge_b_order])))))
+QED;
+
 (* Translations *)
-val _ = translate leaf_def;
+val _ = translate leaf_def;b_f
 val _ = translate root_def;
 val _ = translate rank_def;
 val _ = translate aux_def;
